post-cip/formal-crypto/lean/src/Leioscrypto/Vote.lean
@@ -39,29 +39,79 @@ namespace Vote
     correct_block : vote.ebHash = election.ebHash
     valid_pool :
       match vote with
-      | PersistentVote _ poolIndex _ _ => election.epoch.valid_index poolIndex
-      | NonpersistentVote _ poolId _ _ _ => election.epoch.valid_poolid poolId
+      | PersistentVote _ poolIndex _ _ => election.epoch.fa.valid_persistent_poolindex poolIndex
+      | NonpersistentVote _ poolId _ _ _ => election.epoch.fa.valid_nonpersistent_poolid poolId
 
-  def lookupPool (election : Election) (vote : Vote) (valid : vote.Valid election) : PoolKeyHash :=
-    match vote with
-    | PersistentVote _ poolIndex _ _ => election.epoch.stakes.lookupPoolId poolIndex valid.valid_pool
-    | NonpersistentVote _ poolId _ _ _ => poolId
+  private def AuthenticPersistent (election : Election) (poolIndex : PoolIndex) (σ_m : BLS.Signature) (h: election.epoch.fa.valid_persistent_poolindex poolIndex) : Prop :=
+    let epoch := election.epoch
+    let fa := epoch.fa
+    let stakes := fa.stakes
+    let registry := epoch.registry
+    let validIndex : stakes.valid_poolindex poolIndex :=
+      by
+        apply fa.persistent_index_is_valid_index
+        apply h
+    let poolId : PoolKeyHash := stakes.lookupPoolId poolIndex validIndex
+    let validId : registry.valid_poolid poolId := epoch.valid_persistent_index_in_registry poolIndex h validIndex
+    let registration : Registration := registry.lookupRegistration poolId validId
+    let eid := election.electionId.toByteArray
+    let mvk := registration.pool.mvk
+    let msg_m := eid ++ election.ebHash.toByteArray
+    let ver_m := BLS.Ver mvk msg_m σ_m
+    let weight : Rat := fa.persistentWeight poolIndex h
+    let hasSeats := weight > 0
+    ver_m ∧ hasSeats
+
+  private def AuthenticNonpersistent (election : Election) (poolId : PoolKeyHash) (σ_eid : BLS.Signature) (σ_m : BLS.Signature) (h: election.epoch.fa.valid_nonpersistent_poolid poolId) : Prop :=
+    let epoch := election.epoch
+    let fa := epoch.fa
+    let stakes := fa.stakes
+    let registry := epoch.registry
+    let validId : registry.valid_poolid poolId :=
+      by
+        apply epoch.valid_nonpersistent_id_in_registry
+        apply h
+    let registration : Registration := registry.lookupRegistration poolId validId
+    let mvk := registration.pool.mvk
+    let eid := election.electionId.toByteArray
+    let msg_eid := eid ++ election.epoch.nonce.toByteArray
+    let ver_eid := BLS.Ver mvk msg_eid σ_eid
+    let msg_m := eid ++ election.ebHash.toByteArray
+    let ver_m := BLS.Ver mvk msg_m σ_m
+    let weight : Rat := fa.nonpersistentWeight poolId h.valid₁ σ_eid
+    let hasSeats := weight > 0
+    ver_eid ∧ ver_m ∧ hasSeats
 
   def Authentic (election : Election) (vote : Vote) (valid : vote.Valid election) : Prop :=
+    match vote with
+    | PersistentVote _ poolIndex _ σ_m => AuthenticPersistent election poolIndex σ_m $ by apply valid.valid_pool
+    | NonpersistentVote _ poolId σ_eid _ σ_m => AuthenticNonpersistent election poolId σ_eid σ_m $ by apply valid.valid_pool
+    /-
     let epoch := election.epoch
+    let fa := epoch.fa
+    let stakes := fa.stakes
     let registry := epoch.registry
+    let h₁ : ∃ poolId : PoolKeyHash, registry.valid_poolid poolId :=
+     sorry
     let poolId := vote.lookupPool election valid
-    let validId : poolId ∈ registry.map Registration.poolId :=
+    let validId : registry.valid_poolid poolId :=
      by
       cases vote
       case PersistentVote _ poolIndex _ _ =>
-        apply epoch.pools_valid_ids
-        let h₁ := valid.valid_pool
-        simp [*] at h₁
-        apply epoch.stakes.poolindex_in_pools poolIndex h₁
+        have h₁ : fa.valid_persistent_poolindex poolIndex :=
+          by
+            apply valid.valid_pool
+        obtain ⟨ _ , h₂ ⟩ := epoch.valid_persistent_index_in_registry poolIndex h₁
+
+        --apply vote.lookupPool at poolId
+        sorry
       case NonpersistentVote _ _ _ _ _ =>
-        apply epoch.pools_valid_ids
-        apply valid.valid_pool
+        have h₁ : fa.valid_nonpersistent_poolid poolId :=
+          by
+            sorry
+        let x := epoch.valid_nonpersistent_id_in_registry h₁
+        exact x
+        sorry
     let registration : Registration := registry.lookupRegistration poolId validId
     let mvk := registration.pool.mvk
     let eid := election.electionId.toByteArray
@@ -71,9 +121,15 @@ namespace Vote
     let ver_m := BLS.Ver mvk msg_m vote.σ_m
     let has_seats := epoch.fa.voteWeight poolId vote.σ_eid ≠ none
     ver_eid ∧ ver_m ∧ has_seats
+    -/
 
     def Checked (election : Election) (vote : Vote) (valid : vote.Valid election) : Prop :=
       vote.WellFormed ∧ vote.Authentic election valid
+
+    structure Checked' (election : Election) (vote : Vote) : Prop where
+      wf : vote.WellFormed
+      valid : vote.Valid election
+      authentic: vote.Authentic election valid
 
 end Vote
 
